NonHamiltonian: Update

NonHamiltonian/Digraph.lean
@@ -6,7 +6,7 @@ Released under Apache 2.0 license as described in the file LICENSE.
 module
 
 public import NonHamiltonian.List
-public import NonHamiltonian.Set
+public import Std.Data.ExtTreeSet
 
 @[expose] public section
 
@@ -15,82 +15,94 @@ public import NonHamiltonian.Set
 set_option autoImplicit false
 
 namespace NonHamiltonian
+universe u
+open Std
 
-abbrev Node           := Nat
-abbrev Edge           := Nat × Nat
-instance : Ord (Edge) := lexOrd
-abbrev NodeSet        := Set Node
-abbrev EdgeSet        := Set Edge
-
-structure Digraph where
-  nodes          : NodeSet
-  edges          : EdgeSet
+/-- Simple directed graph with nodes of a `LawfulEqOrd` type. -/
+structure Digraph (α : Type u) [Ord α] [TransOrd α] [LawfulEqOrd α] where
+  nodes : ExtTreeSet α
+  edges : ExtTreeSet (α × α) lexOrd.compare
   nodes_nonempty : nodes ≠ ∅ := by decide
   edges_endnodes : edges.toList.all (λ (l,r) ↦
     nodes.contains l && nodes.contains r) := by decide
-  deriving Repr, DecidableEq
+  deriving Repr
 
 namespace Digraph
+variable {α : Type u} [Ord α] [TransOrd α] [LawfulEqOrd α]
 
-theorem nodes_size_ne_zero {g : Digraph} : g.nodes.size ≠ 0 := by
+theorem nodes_size_ne_zero {g : Digraph α} : g.nodes.size ≠ 0 := by
   simp [← g.nodes.eq_empty_iff_size_eq_zero, g.nodes_nonempty]
 
-theorem zero_lt_nodes_size {g : Digraph} : 0 < g.nodes.size := by
+theorem zero_lt_nodes_size {g : Digraph α} : 0 < g.nodes.size := by
   rw [← Nat.ne_zero_iff_zero_lt]; exact g.nodes_size_ne_zero
 
-theorem edges_endnodes' {g : Digraph} :
+theorem edges_endnodes' {g : Digraph α} :
     ∀ e ∈ g.edges, e.1 ∈ g.nodes ∧ e.2 ∈ g.nodes := by
   simp only [← g.edges.mem_toList, ← g.nodes.contains_iff_mem,
-    ← Bool.and_eq_true]; exact List.all_eq_true.mp g.edges_endnodes
+    ← Bool.and_eq_true]
+  exact List.all_eq_true.mp g.edges_endnodes
+
+end Digraph
 
 /-! ## Hamiltonian Path -/
 
-structure HamiltonianPath (g : Digraph) where
-  path      : List Node
+/-- A Hamiltonian path in a digraph `g` is a list of nodes `path` such that:
+(i) `path` is a permutation of the nodes of `g`; and
+(ii) there is an edge in `g` for each consecutive pair of nodes in `path`. -/
+structure Digraph.HamiltonianPath
+    {α : Type u} [Ord α] [TransOrd α] [LawfulEqOrd α] (g : Digraph α) where
+  path : List α
   path_perm : path.Perm g.nodes.toList := by decide
   path_conn : path.connect.all g.edges.contains := by decide
-  deriving Repr, DecidableEq
+  deriving Repr
 
-namespace HamiltonianPath
+namespace Digraph.HamiltonianPath
+variable {α : Type u} [Ord α] [TransOrd α] [LawfulEqOrd α]
 
-theorem path_length {g : Digraph} {p : HamiltonianPath g} :
+theorem path_length {g : Digraph α} {p : HamiltonianPath g} :
     p.path.length = g.nodes.size := by
   rw [← g.nodes.length_toList]; exact List.Perm.length_eq p.path_perm
 
-theorem path_nonempty {g : Digraph} {p : HamiltonianPath g} :
+theorem path_nonempty {g : Digraph α} {p : HamiltonianPath g} :
     p.path ≠ [] := by
   apply List.ne_nil_of_length_pos; rw [path_length]
   exact g.zero_lt_nodes_size
 
-theorem path_conn_subset_edges {g : Digraph} {p :HamiltonianPath g} :
+theorem path_conn_subset_edges {g : Digraph α} {p :HamiltonianPath g} :
     p.path.connect.Subset g.edges.toList := by
   intro e; rw [g.edges.mem_toList]; exact List.all_eq_true.mp p.path_conn e
 
-end HamiltonianPath
+end Digraph.HamiltonianPath
 
-def Hamiltonian (g : Digraph) : Prop :=
+/-! ## The Hamiltonian property -/
+
+namespace Digraph
+variable {α : Type u} [Ord α] [TransOrd α] [LawfulEqOrd α]
+
+/-- Logical characterization of the Hamiltonian property. -/
+def Hamiltonian (g : Digraph α) : Prop :=
   Nonempty (HamiltonianPath g)
 
-/-- Tests whether digraph is Hamiltonian. -/
-def isHamiltonian (g : Digraph) : Bool :=
+/-- Algorithmic characterization of the Hamiltonian property. -/
+def isHamiltonian (g : Digraph α) : Bool :=
   g.nodes.toList.perms.any (·.connect.all g.edges.contains)
 
 -- TODO: Relate this to isHamiltonian.
-def findHamiltonianPath? (g : Digraph) : Option (HamiltonianPath g) :=
+def findHamiltonianPath? (g : Digraph α) : Option (HamiltonianPath g) :=
   Id.run do
     for hperm : p in g.nodes.toList.perms do
       if hconn : p.connect.all g.edges.contains then
         return some ⟨p, List.perm_of_mem_perms hperm, hconn⟩
     return none
 
-theorem isHamiltonian_iff_Hamiltonian {g : Digraph} :
+theorem isHamiltonian_iff_Hamiltonian [BEq α] [LawfulBEq α] {g : Digraph α} :
     g.isHamiltonian ↔ g.Hamiltonian := by
   rw [isHamiltonian, List.any_eq_true, Hamiltonian]
   constructor <;> rintro ⟨p, hperm, hconn⟩
   · exact Nonempty.intro ⟨p, List.perm_of_mem_perms hperm, hconn⟩
   · exists p; exact ⟨List.mem_perms_of_perm hperm, hconn⟩
 
-instance (g : Digraph) : Decidable (g.Hamiltonian) :=
+instance [BEq α] [LawfulBEq α] (g : Digraph α) : Decidable (g.Hamiltonian) :=
   decidable_of_iff (g.isHamiltonian) isHamiltonian_iff_Hamiltonian
 
 end Digraph
